src/shim.ml
@@ -27,11 +27,12 @@ module type InterpreterType = sig
 
     val run_v :
       Extract.nat ->
+      Extract.nat ->
       Obj.t * Obj.t Extract.store_record * Extract.frame * administrative_instruction list ->
       (Obj.t * Obj.t Extract.store_record) * Extract.res
 
     val run_step_compat :
-      config_tuple -> Extract.res_tuple
+      int -> config_tuple -> Extract.res_tuple
 
     val is_const_list : administrative_instruction list -> Extract.value0 list option
 
@@ -92,12 +93,12 @@ module Interpreter =
     type res_tuple = Extract.res_tuple
     type administrative_instruction = Extract.administrative_instruction
 
-    let run_v i cfg =
+    let run_v i d cfg =
       let (hs, s, f, es) = cfg in
-      Interpreter.run_v hs s f es i
+      Interpreter.run_v hs s f es i d
 
-    let run_step_compat cfg =
-      Interpreter.run_step_compat cfg
+    let run_step_compat d cfg =
+      Interpreter.run_step_compat (Convert.to_nat d) cfg
 
     let is_const_list = Interpreter.is_const_list
 
