theories/interpreter_func.v
@@ -1,3 +1,606 @@
+(** Wasm interpreter **)
+(* (C) J. Pichon, M. Bodin - see LICENSE.txt *)
+
+From Wasm Require Import common.
+From Coq Require Import ZArith.BinInt.
+From mathcomp Require Import ssreflect ssrfun ssrnat ssrbool eqtype seq.
+From Wasm Require Export operations host type_checker.
+Require Import BinNat.
+
+Set Implicit Arguments.
+Unset Strict Implicit.
+
+Unset Printing Implicit Defensive.
+
+Inductive res_crash : Type :=
+| C_error : res_crash
+| C_exhaustion : res_crash.
+
+Scheme Equality for res_crash.
+Definition res_crash_eqb c1 c2 := is_left (res_crash_eq_dec c1 c2).
+Definition eqres_crashP : Equality.axiom res_crash_eqb :=
+  eq_dec_Equality_axiom res_crash_eq_dec.
+
+Canonical Structure res_crash_eqMixin := EqMixin eqres_crashP.
+Canonical Structure res_crash_eqType := Eval hnf in EqType res_crash res_crash_eqMixin.
+
+Inductive res : Type :=
+| R_crash : res_crash -> res
+| R_trap : res
+| R_value : list value -> res.
+
+Definition res_eq_dec : forall r1 r2 : res, {r1 = r2} + {r1 <> r2}.
+Proof. decidable_equality. Defined.
+
+Definition res_eqb (r1 r2 : res) : bool := res_eq_dec r1 r2.
+Definition eqresP : Equality.axiom res_eqb :=
+  eq_dec_Equality_axiom res_eq_dec.
+
+Canonical Structure res_eqMixin := EqMixin eqresP.
+Canonical Structure res_eqType := Eval hnf in EqType res res_eqMixin.
+
+Section Host_func.
+
+Variable host_function : eqType.
+Let host := host host_function.
+
+Variable host_instance : host.
+
+Let store_record := store_record host_function.
+(*Let administrative_instruction := administrative_instruction host_function.*)
+Let host_state := host_state host_instance.
+
+(*Let vs_to_es : seq value -> seq administrative_instruction := @vs_to_es _.*)
+
+Variable host_application_impl : host_state -> store_record -> function_type -> host_function -> seq value ->
+                       (host_state * option (store_record * result)).
+
+Hypothesis host_application_impl_correct :
+  (forall hs s ft hf vs hs' hres, (host_application_impl hs s ft hf vs = (hs', hres)) -> host_application hs s ft hf vs hs' hres).
+
+Inductive res_step : Type :=
+| RS_crash : res_crash -> res_step
+| RS_break : nat -> list value -> res_step
+| RS_return : list value -> res_step
+| RS_normal : list administrative_instruction -> res_step.
+
+Definition res_step_eq_dec : forall r1 r2 : res_step, {r1 = r2} + {r1 <> r2}.
+Proof. decidable_equality. Defined.
+
+Definition res_step_eqb (r1 r2 : res_step) : bool := res_step_eq_dec r1 r2.
+Definition eqres_stepP : Equality.axiom res_step_eqb :=
+  eq_dec_Equality_axiom res_step_eq_dec.
+
+Canonical Structure res_step_eqMixin := EqMixin eqres_stepP.
+Canonical Structure res_step_eqType := Eval hnf in EqType res_step res_step_eqMixin.
+
+Definition crash_error := RS_crash C_error.
+
+Definition depth := nat.
+
+Definition fuel := nat.
+
+Definition config_tuple := ((host_state * store_record * frame * list administrative_instruction)%type).
+
+Definition config_one_tuple_without_e := (host_state * store_record * frame * list value)%type.
+
+Definition res_tuple := (host_state * store_record * frame * res_step)%type.
+(*
+Fixpoint split_vals (es : list basic_instruction) : ((list value) * (list basic_instruction))%type :=
+  match es with
+  | (EConst v) :: es' =>
+    let: (vs', es'') := split_vals es' in
+    (v :: vs', es'')
+  | _ => ([::], es)
+  end.
+
+(** [split_vals_e es]: takes the maximum initial segment of [es] whose elements
+    are all of the form [AI_basic (EConst v)];
+    returns a pair of lists [(ves, es')] where [ves] are those [v]'s in that initial
+    segment and [es] is the remainder of the original [es]. **)
+Fixpoint split_vals_e (es : list administrative_instruction) : ((list value) * (list administrative_instruction))%type :=
+  match es with
+  | (AI_basic (EConst v)) :: es' =>
+    let: (vs', es'') := split_vals_e es' in
+    (v :: vs', es'')
+  | _ => ([::], es)
+  end.
+
+Fixpoint split_n (es : list value) (n : nat) : ((list value) * (list value))%type :=
+  match (es, n) with
+  | ([::], _) => ([::], [::])
+  | (_, 0) => ([::], es)
+  | (e :: esX, n.+1) =>
+    let: (es', es'') := split_n esX n in
+    (e :: es', es'')
+  end.
+
+Definition expect {A B : Type} (ao : option A) (f : A -> B) (b : B) : B :=
+  match ao with
+  | Some a => f a
+  | None => b
+  end.
+
+Definition vs_to_es (vs : list value) : list administrative_instruction :=
+  v_to_e_list (rev vs).
+
+Definition e_is_trap (e : administrative_instruction) : bool :=
+  match e with
+  | AI_trap => true
+  | _ => false
+  end.
+
+Lemma e_is_trapP : forall e, reflect (e = AI_trap) (e_is_trap e).
+Proof.
+  case => //= >; by [ apply: ReflectF | apply: ReflectT ].
+Qed.
+
+(** [es_is_trap es] is equivalent to [es == [:: AI_trap]]. **)
+Definition es_is_trap (es : list administrative_instruction) : bool :=
+  match es with
+  | [::e] => e_is_trap e
+  | _ => false
+  end.
+
+Lemma es_is_trapP : forall l, reflect (l = [::AI_trap]) (es_is_trap l).
+Proof.
+  case; first by apply: ReflectF.
+  move=> // a l. case l => //=.
+  - apply: (iffP (e_is_trapP _)); first by elim.
+    by inversion 1.
+  - move=> >. by apply: ReflectF.
+Qed.*)
+
+Fixpoint run_step_with_fuel (fuel : fuel) (d : depth) (cfg : config_tuple) : res_tuple :=
+  let: (hs, s, f, es) := cfg in
+  match fuel with
+  | 0 => (hs, s, f, RS_crash C_exhaustion)
+  | fuel.+1 =>
+    let: (ves, es') := split_vals_e es in (** Framing out constants. **)
+    match es' with
+    | [::] => (hs, s, f, crash_error)
+    | e :: es'' =>
+      if e_is_trap e
+      then
+        if (es'' != [::]) || (ves != [::])
+        then (hs, s, f, RS_normal [::AI_trap])
+        else (hs, s, f, crash_error)
+      else
+        let: (hs', s', f', r) := run_one_step fuel d (hs, s, f, (rev ves)) e in
+        if r is RS_normal res
+        then (hs', s', f', RS_normal (res ++ es''))
+        else (hs', s', f', r)
+    end
+  end
+    
+with run_one_step (fuel : fuel) (d : depth) (cfg : config_one_tuple_without_e) (e : administrative_instruction) : res_tuple :=
+  let: (hs, s, f, ves) := cfg in
+  match fuel with
+  | 0 => (hs, s, f, RS_crash C_exhaustion)
+  | fuel.+1 =>
+    match e with
+    (* unop *)
+    | AI_basic (BI_unop t op) =>
+      if ves is v :: ves' then
+        (hs, s, f, RS_normal (vs_to_es (app_unop op v :: ves')))
+      else (hs, s, f, crash_error)
+    (* binop *)
+    | AI_basic (BI_binop t op) =>
+      if ves is v2 :: v1 :: ves' then
+        expect (app_binop op v1 v2)
+               (fun v => (hs, s, f, RS_normal (vs_to_es (v :: ves'))))
+               (hs, s, f, RS_normal ((vs_to_es ves') ++ [::AI_trap]))
+      else (hs, s, f, crash_error)
+    (* testops *)
+    | AI_basic (BI_testop T_i32 testop) =>
+      if ves is (VAL_int32 c) :: ves' then
+        (hs, s, f, RS_normal (vs_to_es ((VAL_int32 (wasm_bool (@app_testop_i i32t testop c))) :: ves')))
+      else (hs, s, f, crash_error)
+    | AI_basic (BI_testop T_i64 testop) =>
+      if ves is (VAL_int64 c) :: ves' then
+        (hs, s, f, RS_normal (vs_to_es ((VAL_int32 (wasm_bool (@app_testop_i i64t testop c))) :: ves')))
+      else (hs, s, f, crash_error)
+    | AI_basic (BI_testop _ _) => (hs, s, f, crash_error)
+    (* relops *)
+    | AI_basic (BI_relop t op) =>
+      if ves is v2 :: v1 :: ves' then
+        (hs, s, f, RS_normal (vs_to_es (VAL_int32 (wasm_bool (app_relop op v1 v2)) :: ves')))
+      else (hs, s, f, crash_error)
+    (* convert & reinterpret *)
+    | AI_basic (BI_cvtop t2 CVO_convert t1 sx) =>
+      if ves is v :: ves' then
+        if types_agree t1 v
+        then
+          expect (cvt t2 sx v) (fun v' =>
+               (hs, s, f, RS_normal (vs_to_es (v' :: ves'))))
+            (hs, s, f, RS_normal ((vs_to_es ves') ++ [::AI_trap]))
+        else (hs, s, f, crash_error)
+      else (hs, s, f, crash_error)
+    | AI_basic (BI_cvtop t2 CVO_reinterpret t1 sx) =>
+      if ves is v :: ves' then
+        if types_agree t1 v && (sx == None)
+        then (hs, s, f, RS_normal (vs_to_es (wasm_deserialise (bits v) t2 :: ves')))
+        else (hs, s, f, crash_error)
+      else (hs, s, f, crash_error)
+    (**)
+    | AI_basic BI_unreachable => (hs, s, f, RS_normal ((vs_to_es ves) ++ [::AI_trap]))
+    | AI_basic BI_nop => (hs, s, f, RS_normal (vs_to_es ves))
+    | AI_basic BI_drop =>
+      if ves is v :: ves' then
+        (hs, s, f, RS_normal (vs_to_es ves'))
+      else (hs, s, f, crash_error)
+    | AI_basic BI_select =>
+      if ves is (VAL_int32 c) :: v2 :: v1 :: ves' then
+        if c == Wasm_int.int_zero i32m
+        then (hs, s, f, RS_normal (vs_to_es (v2 :: ves')))
+        else (hs, s, f, RS_normal (vs_to_es (v1 :: ves')))
+      else (hs, s, f, crash_error)
+    | AI_basic (BI_block (Tf t1s t2s) es) =>
+      if length ves >= length t1s
+      then
+        let: (ves', ves'')  := split_n ves (length t1s) in
+        (hs, s, f, RS_normal (vs_to_es ves''
+                ++ [::AI_label (length t2s) [::] (vs_to_es ves' ++ to_e_list es)]))
+      else (hs, s, f, crash_error)
+    | AI_basic (BI_loop (Tf t1s t2s) es) =>
+      if length ves >= length t1s
+      then
+        let: (ves', ves'') := split_n ves (length t1s) in
+        (hs, s, f, RS_normal (vs_to_es ves''
+                ++ [::AI_label (length t1s) [::AI_basic (BI_loop (Tf t1s t2s) es)]
+                        (vs_to_es ves' ++ to_e_list es)]))
+      else (hs, s, f, crash_error)
+    | AI_basic (BI_if tf es1 es2) =>
+      if ves is VAL_int32 c :: ves' then
+        if c == Wasm_int.int_zero i32m
+        then (hs, s, f, RS_normal (vs_to_es ves' ++ [::AI_basic (BI_block tf es2)]))
+        else (hs, s, f, RS_normal (vs_to_es ves' ++ [::AI_basic (BI_block tf es1)]))
+      else (hs, s, f, crash_error)
+    | AI_basic (BI_br j) => (hs, s, f, RS_break j ves)
+    | AI_basic (BI_br_if j) =>
+      if ves is VAL_int32 c :: ves' then
+        if c == Wasm_int.int_zero i32m
+        then (hs, s, f, RS_normal (vs_to_es ves'))
+        else (hs, s, f, RS_normal (vs_to_es ves' ++ [::AI_basic (BI_br j)]))
+      else (hs, s, f, crash_error)
+    | AI_basic (BI_br_table js j) =>
+      if ves is VAL_int32 c :: ves' then
+        let: k := Wasm_int.nat_of_uint i32m c in
+        if k < length js
+        then
+          expect (List.nth_error js k) (fun js_at_k =>
+              (hs, s, f, RS_normal (vs_to_es ves' ++ [::AI_basic (BI_br js_at_k)])))
+            (hs, s, f, crash_error)
+        else (hs, s, f, RS_normal (vs_to_es ves' ++ [::AI_basic (BI_br j)]))
+      else (hs, s, f, crash_error)
+    | AI_basic (BI_call j) =>
+      if List.nth_error f.(f_inst).(inst_funcs) j is Some a then
+        (hs, s, f, RS_normal (vs_to_es ves ++ [::AI_invoke a]))
+      else (hs, s, f, crash_error)
+    | AI_basic (BI_call_indirect j) =>
+      if ves is VAL_int32 c :: ves' then
+        match stab_addr s f (Wasm_int.nat_of_uint i32m c) with
+        | Some a =>
+          match List.nth_error s.(s_funcs) a with
+          | Some cl =>
+            if stypes s f.(f_inst) j == Some (cl_type cl)
+            then (hs, s, f, RS_normal (vs_to_es ves' ++ [::AI_invoke a]))
+            else (hs, s, f, RS_normal (vs_to_es ves' ++ [::AI_trap]))        
+          | None => (hs, s, f, crash_error)
+          end
+        | None => (hs, s, f, RS_normal (vs_to_es ves' ++ [::AI_trap]))
+        end
+      else (hs, s, f, crash_error)
+    | AI_basic BI_return => (hs, s, f, RS_return ves)
+    | AI_basic (BI_get_local j) =>
+      if j < length f.(f_locs)
+      then
+        expect (List.nth_error f.(f_locs) j) (fun vs_at_j =>
+            (hs, s, f, RS_normal (vs_to_es (vs_at_j :: ves))))
+          (hs, s, f, crash_error)
+      else (hs, s, f, crash_error)
+    | AI_basic (BI_set_local j) =>
+      if ves is v :: ves' then
+        if j < length f.(f_locs)
+        then (hs, s, Build_frame (set_nth v f.(f_locs) j v) f.(f_inst), RS_normal (vs_to_es ves'))
+        else (hs, s, f, crash_error)
+      else (hs, s, f, crash_error)
+    | AI_basic (BI_tee_local j) =>
+      if ves is v :: ves' then
+        (hs, s, f, RS_normal (vs_to_es (v :: ves) ++ [::AI_basic (BI_set_local j)]))
+      else (hs, s, f, crash_error)
+    | AI_basic (BI_get_global j) =>
+      if sglob_val s f.(f_inst) j is Some xx
+      then (hs, s, f, RS_normal (vs_to_es (xx :: ves)))
+      else (hs, s, f, crash_error)
+    | AI_basic (BI_set_global j) =>
+      if ves is v :: ves' then
+        if supdate_glob s f.(f_inst) j v is Some xx
+        then (hs, xx, f, RS_normal (vs_to_es ves'))
+        else (hs, s, f, crash_error)
+      else (hs, s, f, crash_error)
+    | AI_basic (BI_load t None a off) =>
+      if ves is VAL_int32 k :: ves' then
+        expect
+          (smem_ind s f.(f_inst))
+          (fun j =>
+             if List.nth_error s.(s_mems) j is Some mem_s_j then
+               expect
+                 (load (mem_s_j) (Wasm_int.N_of_uint i32m k) off (t_length t))
+                 (fun bs => (hs, s, f, RS_normal (vs_to_es (wasm_deserialise bs t :: ves'))))
+                 (hs, s, f, RS_normal (vs_to_es ves' ++ [::AI_trap]))
+             else (hs, s, f, crash_error))
+          (hs, s, f, crash_error)
+      else (hs, s, f, crash_error)
+    | AI_basic (BI_load t (Some (tp, sx)) a off) =>
+      if ves is VAL_int32 k :: ves' then
+        expect
+          (smem_ind s f.(f_inst))
+          (fun j =>
+             if List.nth_error s.(s_mems) j is Some mem_s_j then
+               expect
+                 (load_packed sx (mem_s_j) (Wasm_int.N_of_uint i32m k) off (tp_length tp) (t_length t))
+                 (fun bs => (hs, s, f, RS_normal (vs_to_es (wasm_deserialise bs t :: ves'))))
+                 (hs, s, f, RS_normal (vs_to_es ves' ++ [::AI_trap]))
+             else (hs, s, f, crash_error))
+          (hs, s, f, crash_error)
+      else (hs, s, f, crash_error)
+    | AI_basic (BI_store t None a off) =>
+      if ves is v :: VAL_int32 k :: ves' then
+        if types_agree t v
+        then
+          expect
+            (smem_ind s f.(f_inst))
+            (fun j =>
+               if List.nth_error s.(s_mems) j is Some mem_s_j then
+                 expect
+                   (store mem_s_j (Wasm_int.N_of_uint i32m k) off (bits v) (t_length t))
+                   (fun mem' =>
+                      (hs, upd_s_mem s (set_nth mem' s.(s_mems) j mem'), f, RS_normal (vs_to_es ves')))
+                   (hs, s, f, RS_normal (vs_to_es ves' ++ [::AI_trap]))
+               else (hs, s, f, crash_error))
+            (hs, s, f, crash_error)
+        else (hs, s, f, crash_error)
+      else (hs, s, f, crash_error)
+    | AI_basic (BI_store t (Some tp) a off) =>
+      if ves is v :: VAL_int32 k :: ves' then
+        if types_agree t v
+        then
+          expect
+            (smem_ind s f.(f_inst))
+            (fun j =>
+               if List.nth_error s.(s_mems) j is Some mem_s_j then
+                 expect
+                   (store_packed mem_s_j (Wasm_int.N_of_uint i32m k) off (bits v) (tp_length tp))
+                   (fun mem' =>
+                      (hs, upd_s_mem s (set_nth mem' s.(s_mems) j mem'), f, RS_normal (vs_to_es ves')))
+                   (hs, s, f, RS_normal (vs_to_es ves' ++ [::AI_trap]))
+               else (hs, s, f, crash_error))
+            (hs, s, f, crash_error)
+        else (hs, s, f, crash_error)
+      else (hs, s, f, crash_error)
+    | AI_basic BI_current_memory =>
+      expect
+        (smem_ind s f.(f_inst))
+        (fun j =>
+           if List.nth_error s.(s_mems) j is Some s_mem_s_j then
+             (hs, s, f, RS_normal (vs_to_es (VAL_int32 (Wasm_int.int_of_Z i32m (Z.of_nat (mem_size s_mem_s_j))) :: ves)))
+           else (hs, s, f, crash_error))
+        (hs, s, f, crash_error)
+    | AI_basic BI_grow_memory =>
+      if ves is VAL_int32 c :: ves' then
+        expect
+          (smem_ind s f.(f_inst))
+          (fun j =>
+            if List.nth_error s.(s_mems) j is Some s_mem_s_j then
+              let: l := mem_size s_mem_s_j in
+              let: mem' := mem_grow s_mem_s_j (Wasm_int.N_of_uint i32m c) in
+              if mem' is Some mem'' then
+                (hs, upd_s_mem s (set_nth mem'' s.(s_mems) j mem''), f,
+                 RS_normal (vs_to_es (VAL_int32 (Wasm_int.int_of_Z i32m (Z.of_nat l)) :: ves')))
+              else (hs, s, f, crash_error)
+            else (hs, s, f, crash_error))
+          (hs, s, f, crash_error)
+      else (hs, s, f, crash_error)
+    | AI_basic (BI_const _) => (hs, s, f, crash_error)
+    | AI_invoke a =>
+      match List.nth_error s.(s_funcs) a with
+      | Some cl => 
+        match cl with
+        | FC_func_native i (Tf t1s t2s) ts es =>
+            let: n := length t1s in
+            let: m := length t2s in
+            if length ves >= n
+            then
+            let: (ves', ves'') := split_n ves n in
+            let: zs := n_zeros ts in
+            (hs, s, f, RS_normal (vs_to_es ves''
+                    ++ [::AI_local m (Build_frame (rev ves' ++ zs) i) [::AI_basic (BI_block (Tf [::] t2s) es)]]))
+            else (hs, s, f, crash_error)
+        | FC_func_host (Tf t1s t2s) cl' =>
+            let: n := length t1s in
+            let: m := length t2s in
+            if length ves >= n
+            then
+            let: (ves', ves'') := split_n ves n in
+            match host_application_impl hs s (Tf t1s t2s) cl' (rev ves') with
+            | (hs', Some (s', rves)) =>
+                (hs', s', f, RS_normal (vs_to_es ves'' ++ (result_to_stack rves)))
+            | (hs', None) => (hs', s, f, RS_normal (vs_to_es ves ++ [::AI_invoke a]))
+            end
+            else (hs, s, f, crash_error)
+        end
+      | None => (hs, s, f, crash_error)
+      end
+    | AI_label ln les es =>
+      if es_is_trap es
+      then (hs, s, f, RS_normal (vs_to_es ves ++ [::AI_trap]))
+      else
+        if const_list es
+        then (hs, s, f, RS_normal (vs_to_es ves ++ es))
+        else
+          let: (hs', s', f', res) := run_step_with_fuel fuel d (hs, s, f, es) in
+          match res with
+          | RS_break 0 bvs =>
+            if length bvs >= ln
+            then (hs', s', f', RS_normal ((vs_to_es ((take ln bvs) ++ ves)) ++ les))
+            else (hs', s', f', crash_error)
+          | RS_break (n.+1) bvs => (hs', s', f', RS_break n bvs)
+          | RS_return rvs => (hs', s', f', RS_return rvs)
+          | RS_normal es' =>
+            (hs', s', f', RS_normal (vs_to_es ves ++ [::AI_label ln les es']))
+          | RS_crash error => (hs', s', f', RS_crash error)
+          end
+    | AI_local ln lf es =>
+      if es_is_trap es
+      then (hs, s, f, RS_normal (vs_to_es ves ++ [::AI_trap]))
+      else
+        if const_list es
+        then
+          if length es == ln
+          then (hs, s, f, RS_normal (vs_to_es ves ++ es))
+          else (hs, s, f, crash_error)
+        else
+          let: (hs', s', f', res) := run_step_with_fuel fuel d (hs, s, lf, es) in
+          match res with
+          | RS_return rvs =>
+            if length rvs >= ln
+            then (hs', s', f, RS_normal (vs_to_es (take ln rvs ++ ves)))
+            else (hs', s', f, crash_error)
+          | RS_normal es' =>
+            (hs', s', f, RS_normal (vs_to_es ves ++ [::AI_local ln f' es']))
+          | RS_crash error => (hs', s', f, RS_crash error)
+          | RS_break _ _ => (hs', s', f, crash_error)
+          end
+    | AI_trap => (hs, s, f, crash_error)
+    end
+  end.
+
+(** Enough fuel so that [run_one_step] does not run out of exhaustion. **)
+Definition run_one_step_fuel : administrative_instruction -> nat.
+Proof.
+  move=> es. induction es using administrative_instruction_rect';
+    let rec aux v :=
+      lazymatch goal with
+      | F : TProp.Forall _ _ |- _ =>
+        apply TProp.max in F;
+        move: F;
+        let n := fresh "n" in
+        move=> n;
+        aux (n + v)
+      | |- _ => exact (v.+1)
+      end in
+    aux (1 : nat).
+Defined.
+
+(** Enough fuel so that [run_step] does not run out of exhaustion. **)
+Definition run_step_fuel (cfg : config_tuple) : nat :=
+  let: (hs, s, f, es) := cfg in
+  1 + List.fold_left max (List.map run_one_step_fuel es) 0.
+
+Definition run_step (d : depth) (cfg : config_tuple) : res_tuple :=
+  run_step_with_fuel (run_step_fuel cfg) d cfg.
+
+Definition run_step_compat (d: depth) (cfg : config_tuple) : res_tuple :=
+  run_step d cfg.
+  (*let: (hs, s, f, es) := cfg in
+  match run_step_with_measure hs s f es with
+  | RS'_normal hs' s' f' es' _ => (hs', s', f', RS_normal es')
+  | _ => (hs, s, f, RS_crash C_error)
+  end.*)
+
+Fixpoint run_v hs s f es (fuel : fuel) (d : depth) : ((host_state * store_record * res)%type) :=
+  match fuel with
+  | 0 => (hs, s, R_crash C_exhaustion)
+  | fuel.+1 =>
+    if es_is_trap es
+    then (hs, s, R_trap)
+    else
+      if const_list es
+      then (hs, s, R_value (fst (split_vals_e es)))
+      else
+        let: (hs', s', f', res) := run_step d (hs, s, f, es) in
+        match res with
+        | RS_normal es' => run_v hs' s' f' es' fuel d
+        | RS_crash error => (hs', s', R_crash error)
+        | _ => (hs', s', R_crash C_error)
+        end
+  end.
+
+End Host_func.
+
+
+
+Module EmptyHost.
+
+Definition host_function := void.
+
+Definition host_function_eq_dec : forall f1 f2 : host_function, {f1 = f2} + {f1 <> f2}.
+Proof. decidable_equality. Defined.
+
+Definition host_function_eqb f1 f2 : bool := host_function_eq_dec f1 f2.
+Definition host_functionP : Equality.axiom host_function_eqb :=
+  eq_dec_Equality_axiom host_function_eq_dec.
+
+Canonical Structure host_function_eqMixin := EqMixin host_functionP.
+Canonical Structure host_function_eqType :=
+  Eval hnf in EqType host_function host_function_eqMixin.
+
+Definition host : Type := host host_function_eqType.
+
+Definition store_record := store_record host_function_eqType.
+Definition function_closure := function_closure host_function_eqType.
+
+Definition host_instance : host.
+Proof.
+  by refine {|
+      host_state := unit_eqType ;
+      host_application _ _ _ _ _ _ _ := False
+    |}; intros; exfalso; auto.
+Defined.
+
+Definition config_tuple := config_tuple host_instance.
+Definition res_tuple := res_tuple host_instance.
+
+Definition host_state := host_state host_instance.
+
+End EmptyHost.
+
+
+
+Module Interpreter_func_extract.
+
+Export EmptyHost.
+
+Definition host_application_impl : host_state -> store_record -> function_type -> host_function_eqType -> seq value ->
+                                   (host_state * option (store_record * result)).
+Proof.
+  move => ??? hf; by inversion hf.
+Defined.
+
+Definition host_application_impl_correct :
+  (forall hs s ft hf vs hs' hres, (host_application_impl hs s ft hf vs = (hs', hres)) -> host_application hs s ft hf vs hs' hres).
+Proof.
+  move => ??? hf; by inversion hf.
+Defined.
+
+Definition run_v := run_v host_application_impl.
+
+Definition run_step := run_step host_application_impl.
+
+Definition run_step_compat := run_step_compat host_application_impl.
+
+(** State whether a list of administrative instruction is a final value. **)
+Definition is_const_list : list administrative_instruction -> option (list value) :=
+  @those_const_list.
+
+End Interpreter_func_extract.
+
+
+
+
+(*
+
 (** Proof-carrying interpreter for Wasm **)
 
 From Wasm Require Import common opsem properties tactic typing_inversion.
@@ -2897,9 +3500,6 @@ Defined.
 Definition run_step_with_measure hs s f es :=
   @run_step (run_step_measure es) hs s f es (Logic.eq_refl (run_step_measure es)).
 
-
-
-
 (* Extracting a pure interpreter without proofs *)
 Inductive res_step : Type :=
 | RS_crash : res_crash -> res_step
@@ -3060,3 +3660,6 @@ Definition is_const_list : list administrative_instruction -> option (list value
   @those_const_list.
 
 End Interpreter_func_extract.
+
+
+*)
